WIP on tstack

src/example/TreiberStackSpec.v
@@ -7,91 +7,195 @@ From Fairness Require Import FairBeh Mod Linking.
 From Fairness Require Import TreiberStack.
 From Fairness Require Import PCM IProp IPM IPropAux.
 From Fairness Require Import IndexedInvariants OpticsInterp SimWeakest.
-From Fairness Require Import TemporalLogic SCMemSpec AuthExclsRA.
+From Fairness Require Import TemporalLogic SCMemSpec AuthExclsRA ghost_map ExclsRA.
 
+Record maybe_null_ptr := {
+  ptr :> SCMem.val;
+  ptr_mabye_null : ptr = SCMem.val_null \/ (∃ (p : SCMem.pointer), ptr = SCMem.val_ptr p);
+}.
+Global Instance maybe_null_ptr_eq_dec : EqDecision maybe_null_ptr.
+Proof.
+  intros [p1 Pp1] [p2 Pp2].
+  unfold Decision. destruct (decide (p1 = p2)) as [->|NEQ].
+  - left. f_equal. apply proof_irrelevance.
+  - right. intros H. apply NEQ. injection H. done.
+Qed.
+
+Definition to_mnp_null : maybe_null_ptr := {| ptr := SCMem.val_null; ptr_mabye_null := or_introl eq_refl |}.
+
+Definition to_mnp_ptr ptr
+  (IsPtr : (∃ (p : SCMem.pointer), ptr = SCMem.val_ptr p)) :=
+  {| ptr := ptr; ptr_mabye_null := or_intror IsPtr |}.
+
+Module TreiberStackSpec.
 Section SPEC.
 
   Context {src_state : Type}.
   Context {src_ident : Type}.
   Context {Client : Mod.t}.
   Context {gvs : list nat}.
-  Context (treiberN : namespace).
+  Context (treiberN : namespace) `{DISJ: (↑N_state_tgt :coPset) ## (↑treiberN : coPset)}.
   Notation tgt_state := (OMod.closed_state Client (SCMem.mod gvs)).
   Notation tgt_ident := (OMod.closed_ident Client (SCMem.mod gvs)).
 
   Local Instance STT : StateTypes := Build_StateTypes src_state tgt_state src_ident tgt_ident.
+
   Context `{sub : @SRA.subG Γ Σ}.
   Context {TLRASs : TLRAs_small STT Γ}.
   Context {TLRAS : TLRAs STT Γ Σ}.
 
   Context {HasMEMRA: @GRA.inG memRA Γ}.
-  Context {HasAuthExclAnys : @GRA.inG (AuthExcls.t (list SCMem.val)) Γ}.
+  Context {HasAuthExcl : @GRA.inG (AuthExcls.t (list SCMem.val)) Γ}.
+  Context {HasExcl : @GRA.inG (Excls.t unit) Γ}.
+  Context {HasGhostMap : @GRA.inG (ghost_mapURA nat maybe_null_ptr) Γ}.
 
-  Ltac red_tl_all := red_tl; red_tl_memra; red_tl_authexcls.
+  Ltac red_tl_all := red_tl_every; red_tl_memra; red_tl_authexcls; red_tl_ghost_map_ura.
 
-  Inductive mabye_null_ptr : Type :=
-  | Null
-  | Ptr (p : SCMem.pointer).
-  Local Instance mabye_null_ptr_eqdec : EqDecision mabye_null_ptr.
-  Proof. solve_decision. Qed.
+  Definition to_val (mnp : maybe_null_ptr) : SCMem.val :=
+    ptr mnp.
 
-  Definition to_val (mnp : mabye_null_ptr) : SCMem.val :=
-    match mnp with
-    | Null => SCMem.val_null
-    | Ptr p => SCMem.val_ptr p
-    end.
-
-  Fixpoint phys_list n (l : mabye_null_ptr) (L : list SCMem.val) : sProp n := (
-    match (l,L) with
-    | (Null, []) => emp
-    | (Null, _ :: _) => ⌜False⌝
-    | (Ptr _, []) => ⌜False⌝
-    | (Ptr l, v::tL) => ∃ (r : τ{mabye_null_ptr}), (l ↦∗□ [(to_val r); v]) ∗ (phys_list n r tL)
+  Fixpoint phys_list n (l : maybe_null_ptr) (L : list SCMem.val) : sProp n := (
+    match L with
+    | [] => ⌜to_val l = SCMem.val_null⌝
+    | v::tL => ∃ (p : τ{SCMem.pointer}) (r : τ{maybe_null_ptr}), ⌜to_val l = SCMem.val_ptr p⌝ ∗ (l ↦∗□ [(to_val r); v]) ∗ (phys_list n r tL)
     end
   )%S.
 
-  Definition TStackLivenessInv (lv k γs : nat) (h : mabye_null_ptr) : sProp (1+lv)  := (
-    ∃ (m : τ{ (gmap nat (option mabye_null_ptr)) ,1+lv}),
-    [∗ (1+lv) , (option mabye_null_ptr) map] i ↦ op ∈ m, (
-      match op with
-      | None => emp
-      | Some p =>
-        if (decide (h=p)) then
-          ◇[k](0,1)
-        else
-          emp
-      end
+  Definition LInv (n k γs : nat) (h : maybe_null_ptr) (m : gmap nat maybe_null_ptr) : sProp n  := (
+    s_ghost_map_auth γs 1 m ∗
+    [∗ n, maybe_null_ptr map] i ↦ p ∈ m, (
+      if (decide (h=p)) then
+        emp
+      else
+        ◇[k](0,1)
     )
   )%S.
 
-  (* Definition TreiberStackInv (n : nat) (s : SCMem.val) (γs : nat) : sProp n := (
-    ∃ (h : τ{option SCMem.pointer}) (L : τ{list SCMem.val}),
+  Definition Inv (n : nat) (s : SCMem.val) (k γs : nat) : sProp n := (
+    ∃ (h : τ{maybe_null_ptr}) (L : τ{list SCMem.val}) (m : τ{gmap nat maybe_null_ptr,n}),
       s ↦ (to_val h) ∗ ● γs (L : list SCMem.val) ∗
-      phys_list n h L ∗
+      phys_list n h L ∗ LInv n k γs h m
   )%S.
 
-  Definition IsTreiber n s γs : sProp n := (
-    syn_inv n treiberN (TreiberStackInv n s γs)
+  Definition IsT n s k γs : sProp n := (
+    syn_inv n treiberN (Inv n s k γs)
   )%S.
 
-  Global Instance IsTreiber_persistent n s γs:
-    Persistent (⟦ IsTreiber n s γs, n⟧).
-  Proof. unfold Persistent,IsTreiber. rewrite red_syn_inv. by iIntros "#?". Qed.
+  Global Instance IsT_persistent n s k γs :
+    Persistent (⟦ IsT n s k γs, n⟧).
+  Proof. unfold Persistent,IsT. rewrite red_syn_inv. by iIntros "#?". Qed.
 
-  Lemma Treiber_push_spec {n} (E : coPset) (Q : SCMem.val → sProp n) (P : sProp n) tid (SUBSET : (↑treiberN) ⊆ E) :
-    ∀ s γs val L (ds : list (nat * nat * sProp n)),
-    ⊢ [@ tid, n, E @]
+  (* Lemma isSpinlock_unfold n x γx γe k L :
+    (⟦isSpinlock n x γx γe k L, n⟧) -∗ (◆[k, L] ∗ inv n N_Spinlock (spinlockInv n x γx γe)).
+  Proof.
+    iEval (unfold isSpinlock; red_tl). iIntros "[LO INV]". eauto.
+  Qed. *)
+
+  Lemma Inv_unfold n s k γs :
+    (⟦ Inv n s k γs, n ⟧) -∗
+    (∃ (h : τ{maybe_null_ptr,n}) (L : τ{list SCMem.val,n}) (m : τ{gmap nat maybe_null_ptr,n}),
+      (s ↦ (to_val h)) ∗ (● γs (L : list SCMem.val)) ∗
+      ⟦ (phys_list n h L), n⟧ ∗ ⟦ LInv n k γs h m, n⟧).
+  Proof.
+    unfold Inv. iIntros "Inv".
+    repeat (red_tl; iDestruct "Inv" as "[% Inv]").
+    red_tl_all. eauto.
+  Qed.
+
+  Lemma Inv_fold n s k γs h L m :
+    (s ↦ (to_val h)) -∗ (● γs (L : list SCMem.val)) -∗
+    ⟦ (phys_list n h L), n⟧ -∗ ⟦ LInv n k γs h m, n⟧
+    -∗ (⟦ Inv n s k γs, n ⟧).
+  Proof.
+    unfold Inv. iIntros "? ? ? ?".
+    repeat (red_tl; iExists _).
+    red_tl_all. iFrame.
+  Qed.
+
+  Lemma LInv_unfold n k γs h m :
+    (⟦ LInv n k γs h m, n ⟧) -∗
+    (ghost_map_auth γs 1 m ∗
+    [∗ map] a ∈ m,
+      ⟦(if decide (h = a) then
+          emp
+        else
+          ◇[k](0, 1)
+        )%S,n ⟧).
+  Proof.
+    unfold LInv. iIntros "H". red_tl_all.
+    rewrite red_syn_big_sepM. done.
+  Qed.
+
+  Lemma LInv_fold n k γs h m :
+    ghost_map_auth γs 1 m -∗
+    ([∗ map] a ∈ m,
+      ⟦(if decide (h = a) then
+          emp
+        else
+          ◇[k](0, 1)
+        )%S,n ⟧)
+    -∗ (⟦ LInv n k γs h m, n ⟧).
+  Proof.
+    unfold LInv. iIntros "? ?". red_tl_all.
+    rewrite red_syn_big_sepM. iFrame.
+  Qed.
+
+  Lemma phys_list_unfold n l L :
+    (⟦ phys_list n l L, n ⟧) -∗
+    match L with
+    | [] => ⌜to_val l = SCMem.val_null⌝
+    | v::tL => ∃ (p : τ{SCMem.pointer,n}) (r : τ{maybe_null_ptr,n}), ⌜to_val l = SCMem.val_ptr p⌝ ∗ (l ↦∗□ [(to_val r); v]) ∗ (⟦phys_list n r tL,n⟧)
+    end.
+  Proof.
+    iIntros "H". des_ifs. simpl.
+    red_tl_all; iDestruct "H" as "[%x H]".
+    red_tl_all; iDestruct "H" as "[%r H]".
+    red_tl_all; iDestruct "H" as "[%EQ [(l.n↦ & l.d↦ & _) Phys]]".
+    iExists _,_. iFrame. done.
+  Qed.
+
+  Lemma phys_list_fold n l L :
+    (match L with
+    | [] => ⌜to_val l = SCMem.val_null⌝
+    | v::tL => ∃ (p : τ{SCMem.pointer,n}) (r : τ{maybe_null_ptr,n}), ⌜to_val l = SCMem.val_ptr p⌝ ∗ (l ↦∗□ [(to_val r); v]) ∗ (⟦phys_list n r tL,n⟧)
+    end) -∗
+    ⟦ phys_list n l L, n ⟧.
+  Proof.
+    iIntros "H". des_ifs. simpl.
+    red_tl_all; iDestruct "H" as "[%x [%r [%EQ [(l.n↦ & l.d↦ & _) Phys]]]]".
+    red_tl_all. iExists x. red_tl_all. iExists r.
+    red_tl_all. iFrame. done.
+  Qed.
+
+  Lemma phys_list_get_head n l L :
+    ⟦ phys_list n l L, n ⟧ -∗
+    □ if (decide (to_val l = SCMem.val_null)) then
+        emp
+      else (∃ (r : τ{maybe_null_ptr,n}) (h : τ{SCMem.val,n}),
+                 (l ↦∗□ [(to_val r); h]))
+    .
+  Proof.
+    iIntros "H". iDestruct (phys_list_unfold with "H") as "H". destruct L; try done.
+    all: case_decide; try done.
+    - iDestruct "H" as %EQ. done.
+    - iDestruct "H" as (p r) "[%EQ [#H _]]".
+      red_tl_all. iExists r, v. iFrame "H".
+  Qed.
+
+  Lemma Treiber_push_spec {n} (Q : SCMem.val → sProp n) (P : sProp n) tid :
+    ∀ s k γs val lv (ds : list (nat * nat * sProp n)),
+    ⊢ [@ tid, n, ⊤ @]
           ⧼⟦(
             (syn_tgt_interp_as n sndl (fun m => s_memory_black m))
-            ∗ (⤉ IsTreiber n s γs)
+            ∗ (⤉ IsT n s k γs)
             ∗ (⤉ Duty(tid) ds)
             ∗ (⤉ P)
-            (* TODO: masks? *)
             ∗ (∀ (S : τ{list SCMem.val, 1+n}), (⤉ (● γs (S : list SCMem.val) ∗ P))
-                  =|1+n|={E}=∗ (⤉ (● γs (val::S) ∗ Q val))
+                  =|1+n|={⊤ ∖ ↑treiberN}=∗ (⤉ (● γs (val::S) ∗ Q val))
               )
+            ∗ ◇[k](1,1)
             (* TODO: Proper ord level. *)
-            ∗ ◇{List.map fst ds}(2 + L, 1)
+            ∗ ◇{List.map fst ds}(2 + lv, 1)
             )%S, 1+n⟧⧽
             (OMod.close_itree Client (SCMem.mod gvs) (TreiberStack.push (s,val)))
           ⧼_, ⟦(
@@ -99,6 +203,176 @@ Section SPEC.
             )%S, 1+n⟧⧽
   .
   Proof.
+    ii. iStartTriple. red_tl_all.
+    unfold IsT. rewrite red_syn_tgt_interp_as. rewrite red_syn_inv. simpl.
+    iIntros "(#Mem & #IsT & Duty & P & AU & Ob_k & Pcs) Post".
+    red_tl_all.
+    iEval (unfold TreiberStack.push).
+
+    iMod (pcs_drop _ _ _ _ 1 (100 + 1) with "Pcs") as "Pcs"; [lia|].
+    Unshelve. 2: lia.
+    rred2r.
+
+    iMod ((pcs_decr _ _ 100 1) with "Pcs") as "[Pcs Pcs_Y]"; [lia|].
+    iApply (wpsim_yieldR with "[$Duty $Pcs_Y]"); [lia..|].
+    iIntros "Duty _". rred2r.
+
+    iApply (SCMem_alloc_fun_spec with "[$Mem] [-]"); [lia|set_solver|].
+    iIntros (node) "(n.n↦ & n.d↦ & _)".
+    rred2r. iApply wpsim_tauR. rred2r.
+
+    iMod ((pcs_decr _ _ 99 1) with "Pcs") as "[Pcs Pcs_Y]"; [lia|].
+    iApply (wpsim_yieldR with "[$Pcs_Y $Duty]"); [lia|].
+    iIntros "Duty _".
+    rred2r.
+
+    iApply (SCMem_store_fun_spec with "[$Mem $n.d↦] [-]"); [lia|set_solver|].
+    iIntros (?) "n.d↦". rred2r. iApply wpsim_tauR. rred2r.
+
+    iEval (rewrite unfold_iter_eq). rred2r.
+
+    iMod ((pcs_decr _ _ 98 1) with "Pcs") as "[Pcs Pcs_Y]"; [lia|].
+    iApply (wpsim_yieldR with "[$Pcs_Y $Duty]"); [lia|].
+    iIntros "Duty _". rred2r.
+
+    iInv "IsT" as "Inv" "Close". simpl.
+    iDestruct (Inv_unfold with "Inv") as (h L m) "(s↦ & γs & Phys & LInv)".
+    iApply (SCMem_load_fun_spec with "[$Mem $s↦] [-]"); [lia|solve_ndisj|].
+    iIntros (load_v) "[%EQ s↦]". subst.
+    (* Get proof that h is live for future use. *)
+    iDestruct (phys_list_get_head with "Phys") as "#h↦□".
+
+    (* Register this thread to the current waiting list for h. *)
+    iDestruct (LInv_unfold with "LInv") as "[GMap LivC]".
+    set (i := fresh (dom m)).
+    iMod (ghost_map_insert i h with "[$GMap]") as "[GMap i↪]".
+    { apply not_elem_of_dom. apply is_fresh. }
+
+    (* Close Invs *)
+    iDestruct (LInv_fold with "GMap [LivC]") as "LInv".
+    { rewrite big_sepM_insert; last first.
+      { apply not_elem_of_dom. apply is_fresh. }
+      iFrame. iClear "h↦□". case_decide; done.
+    }
+    iDestruct (Inv_fold with "s↦ γs Phys LInv") as "Inv".
+    iMod ("Close" with "Inv") as "_". move: i => i. clear dependent L m rv. rred2r.
+
+    iApply wpsim_tauR. rred2r.
+
+    iMod ((pcs_decr _ _ 97 1) with "Pcs") as "[Pcs Pcs_Y]"; [lia|].
+    iApply (wpsim_yieldR with "[$Pcs_Y $Duty]"); [lia|].
+    iIntros "Duty _". rred2r.
+
+    iApply (SCMem_store_fun_spec with "[$Mem $n.n↦] [-]"); [lia|solve_ndisj|].
+    iIntros (?) "n.n↦". rred2r. iApply wpsim_tauR. rred2r.
+
+    iMod ((pcs_decr _ _ 96 1) with "Pcs") as "[Pcs Pcs_Y]"; [lia|].
+    iApply (wpsim_yieldR with "[$Pcs_Y $Duty]"); [lia|].
+    iIntros "Duty _".
+    rred2r.
+
+    iMod ((pcs_decr _ _ 95 1) with "Pcs") as "[Pcs Pcs_Y]"; [lia|].
+
+    iInv "IsT" as "Inv" "Close". simpl.
+    iDestruct (Inv_unfold with "Inv") as (h' L m) "(s↦ & γs & Phys & LInv)".
+    iDestruct (phys_list_get_head with "Phys") as "#h'↦□".
+    destruct (decide (h = h')) as [<-|NEQ].
+    { (* Equal, CAS success *)
+      iApply (SCMem_cas_loc_fun_spec_gen with "[$Mem $s↦ h↦□ h'↦□] [-]"); [lia|solve_ndisj| |].
+      { des_ifs.
+        iDestruct "h↦□" as (??) "[h↦□ _]".
+        iSplit; iExists _; iFrame "h↦□".
+      }
+      iClear "h↦□ h'↦□".
+      iIntros (b) "POST".
+      iDestruct "POST" as (u) "(%EQ & s↦ & _ & _)".
+      des_ifs. destruct EQ as [-> ->].
+      iSpecialize ("AU" $! L).
+      iEval (red_tl) in "AU".
+      iEval (rewrite red_syn_fupd) in "AU".
+      iEval (red_tl_all) in "AU".
+      rred2r. iApply wpsim_tauR. rred2r.
+
+      (* Update logical stack state. *)
+      iMod ("AU" with "[$γs $P]") as "[γs Q]".
+
+      (* Update physical stack state. *)
+      iMod (SCMem.points_to_persist with "n.n↦") as "#n.n↦".
+      iMod (SCMem.points_to_persist with "n.d↦") as "#n.d↦".
+      iAssert (⌜∃ p : τ{SCMem.pointer,n}, node = SCMem.val_ptr p⌝)%I as %IsPtr.
+      { destruct node; try done. iPureIntro. eauto. }
+      iAssert (⟦ phys_list n (to_mnp_ptr node IsPtr) (val::L), n⟧)%I with "[Phys]" as "Phys".
+      { iApply phys_list_fold. simpl. des. iExists _,_. iFrame "∗#". done. }
+
+      (* Update liveness invariant *)
+      iDestruct (LInv_unfold with "LInv") as "[GMap LivC]".
+
+      iDestruct (ghost_map_lookup with "GMap i↪") as "%Lookup_i".
+      iMod (ghost_map_delete with "GMap i↪") as "GMap".
+
+      (** Create a big_opM of ◇[k](0,1). *)
+      iMod (pc_drop _ 0 _ _ (size (delete i m)) with "Ob_k") as "Ob_k"; [lia|].
+      Unshelve. 2: lia.
+      iAssert ([∗ map] _ ∈ delete i m, ◇[k](0,1))%I with "[Ob_k]" as "Ob_k".
+      { set (m' := delete i m). move: m' => m'.
+        iClear "Mem IsT n.n↦ n.d↦". clear.
+        simpl in *.
+        iInduction (m') as [|id op m NotIN] "IH" using map_ind.
+        { done. }
+        rewrite big_sepM_insert; [|done].
+        rewrite map_size_insert_None; [|done].
+        iDestruct (pc_split _ _ 1 (size m) with "Ob_k") as "[$ Ob_k]".
+        iApply ("IH" with "Ob_k").
+      }
+
+      (** Add it to the invariant. *)
+      iDestruct (big_sepM_delete with "LivC") as "[_ LivC]"; [apply Lookup_i|].
+      iDestruct (LInv_fold _ _ _ (to_mnp_ptr node IsPtr) with "GMap [LivC Ob_k]") as "LInv".
+      { iDestruct (big_sepM_sep_2 with "LivC Ob_k") as "LivC".
+        iApply (big_sepM_mono with "LivC").
+        iIntros (i' p' Lookup_i') "[H C]". des_ifs.
+      }
+
+      iDestruct (Inv_fold with "[s↦] γs Phys LInv") as "Inv".
+      { unfold to_val. iFrame. }
+      iMod ("Close" with "Inv") as "_". rred2r.
+
+      iApply (wpsim_yieldR with "[$Pcs_Y $Duty]"); [lia|].
+      iIntros "Duty _". rred2r. iApply wpsim_tauR. rred2r.
+      iApply "Post". iFrame.
+    }
+    (* Different, CAS fail *)
+    iApply (SCMem_cas_loc_fun_spec_gen with "[$Mem $s↦ h↦□ h'↦□] [-]"); [lia|solve_ndisj| |].
+    { unfold to_val. des_ifs.
+      1,3: iDestruct "h'↦□" as (??) "[h'↦□ _]".
+      2,3: iDestruct "h↦□" as (??) "[h↦□ _]".
+      all: iSplit; try done; iExists _; iFrame "#".
+    }
+    iClear "h↦□ h'↦□".
+    iIntros (b) "POST".
+    iDestruct "POST" as (u) "(%EQ & s↦ & _ & _)".
+    des_ifs. all: destruct EQ as [-> ->].
+    { exfalso. clear - e NEQ. unfold to_val in e.
+      destruct h as [h Ph],h' as [h' Ph']. simpl in *. clarify.
+      assert (Ph = Ph') as -> by apply proof_irrelevance. done.
+    }
+
+    (* Update liveness invariant *)
+    iDestruct (LInv_unfold with "LInv") as "[GMap LivC]".
+
+    iDestruct (ghost_map_lookup with "GMap i↪") as "%Lookup_i".
+    iMod (ghost_map_delete with "GMap i↪") as "GMap".
+
+    iDestruct (big_sepM_delete with "LivC") as "[iC LivC]"; [apply Lookup_i|].
+    case_decide; [done|].
+    red_tl. simpl.
+    (* TODO: uhh... now what? actually set up induction and stuff. *)
+
+    iDestruct (LInv_fold with "GMap LivC") as "LInv".
+    iDestruct (Inv_fold with "s↦ γs Phys LInv") as "Inv".
+    iMod ("Close" with "Inv") as "_". rred2r.
+
+    iApply wpsim_tauR. rred2r. iApply wpsim_tauR.
   Admitted.
 (*
 ∀ (S : τ{list SCMem.val}), (⤉ (● γs (S : list SCMem.val) ∗ P))
@@ -107,13 +381,13 @@ Section SPEC.
                     (⤉ (● γs (S' : list SCMem.val) ∗ Q (ov : option SCMem.val) ∗ ⌜ov = hd_error S⌝)))
 *)
   Lemma Treiber_pop_spec
-        {n} (E : coPset) (Q : (option SCMem.val) → sProp n) (P : sProp n) tid
+        {n} (Q : (option SCMem.val) → sProp n) (P : sProp n) tid
         (SUBSET : (↑treiberN) ⊆ E) :
-    ∀ s γs L (ds : list (nat * nat * sProp n)),
-    ⊢ [@ tid, n, E @]
+    ∀ s k γs L (ds : list (nat * nat * sProp n)),
+    ⊢ [@ tid, n, ⊤ @]
           ⧼⟦(
             (syn_tgt_interp_as n sndl (fun m => s_memory_black m))
-            ∗ (⤉ IsTreiber n s γs)
+            ∗ (⤉ IsT n s k γs)
             ∗ (⤉ Duty(tid) ds)
             ∗ (⤉ P)
             (* TODO: masks? *)
@@ -133,7 +407,6 @@ Section SPEC.
             )%S, 1+n⟧⧽
   .
   Proof.
-  Admitted. *)
+  Admitted.
 
 End SPEC.
-Global Opaque TreiberStack.push TreiberStack.pop.
